feat: working on verifying that merge is a permutation

src/BlockSort.dfy
@@ -27,12 +27,14 @@
 
 module BlockSortUnbound {
   import opened Std.Relations
+  import Std.Collections.Seq
 
   import opened InsertionSortAdaptive
 
 
   module BlockSortUnboundImpl {
     import opened Std.Relations
+    import Std.Collections.Seq
 
     import opened InsertionSortAdaptive
 
@@ -43,7 +45,6 @@ module BlockSortUnbound {
       requires a.Length <= b.Length
       requires lo < hi <= a.Length
       ensures b[..hi-lo] == a[lo..hi]
-      // ensures forall i | 0 <= i < hi-lo :: b[i] == a[lo+i]
     {
       forall i | 0 <= i < hi-lo {
         b[i] := a[lo+i];
@@ -57,21 +58,53 @@ module BlockSortUnbound {
       ensures leq(a[i], a[j])
     {}
 
+    lemma MultiSetTrippleSlice<A(!new)>(a: seq<A>, lo: nat, hi: nat)
+      requires lo <= hi <= |a|
+      ensures multiset(a[..lo]) + multiset(a[lo..hi]) + multiset(a[hi..]) == multiset(a[..])
+    {
+      assert a[..lo] + a[lo..hi] + a[hi..] == a;
+    }
+
+    lemma MultiSet5Slice<A(!new)>(a: seq<A>, i0: nat, i1: nat, i2: nat, i3: nat)
+      requires i0 <= i1 <= i2 <= i3 <= |a|
+      ensures multiset(a[..i0]) + multiset(a[i0..i1]) + multiset(a[i1..i2]) + multiset(a[i2..i3]) + multiset(a[i3..]) == multiset(a)
+    {
+      assert (a[..i0]) + (a[i0..i1]) + (a[i1..i2]) + (a[i2..i3]) + (a[i3..]) == (a);
+    }
+
+    ghost predicate {:opaque} MultisetInv<A(!new)>(
+      a: array<A>, cache: array<A>, snap: seq<A>,
+      lo: nat, mid: nat, hi: nat,
+      target_i: nat, left_i: nat, right_i: nat)
+      requires lo <= mid <= hi <= a.Length
+      requires lo <= target_i <= hi
+      requires 0 <= left_i <= mid - lo <= cache.Length
+      requires mid <= right_i <= hi
+      reads a, cache
+    {
+      multiset(a[..lo]) + multiset(a[lo..target_i]) + multiset(cache[left_i..mid-lo]) + multiset(a[right_i..hi]) + multiset(a[hi..]) == multiset(snap)
+    }
+
+
     method {:isolate_assertions} Merge<A(!new, ==)>(leq: (A, A) -> bool, a: array<A>, lo: nat, mid: nat, hi: nat, cache: array<A>)
       modifies a
       modifies cache
+
       requires a != cache
       requires TotalOrdering(leq)
       requires lo < mid < hi <= a.Length
       requires SortedBy(leq, a[lo..mid])
       requires SortedBy(leq, a[mid..hi])
       requires a.Length <= cache.Length
+
       ensures SortedBy(leq, a[lo..hi])
-      // ensures multiset(a[lo..hi]) == multiset(old(a[lo..hi]))
+      ensures multiset(a[..]) == multiset(old(a[..]))
     {
       ghost var snap := a[..];
 
       CopySubarray(a, lo, mid, cache);
+
+      ghost var snap_cache := cache[..];
 
       var left_start: nat := 0;
       var left_i: nat := left_start;
@@ -82,6 +115,11 @@ module BlockSortUnbound {
       var target_start: nat := lo;
       var target_i: nat := target_start;
       var target_bound: nat := hi;
+
+      // assert MultisetInv(a, cache, snap, lo, mid, hi, lo, 0, mid) by {
+      //   reveal MultisetInv;
+      //   MultiSet5Slice(a[..], lo, lo, mid, hi);
+      // }
 
       // merging left with right
       while left_i < left_bound && right_i < right_bound
@@ -107,6 +145,8 @@ module BlockSortUnbound {
 
         // target
         invariant SortedBy(leq, a[target_start..target_i])
+
+        // invariant MultisetInv(a, cache, snap, lo, mid, hi, target_i, left_i, right_i)
       {
         if leq(cache[left_i], a[right_i]) {
           a[target_i] := cache[left_i];
@@ -120,7 +160,58 @@ module BlockSortUnbound {
         }
 
         target_i := target_i + 1;
+
+        // assert MultisetInv(a, cache, snap, lo, mid, hi, target_i, left_i, right_i) by {
+        //   reveal MultisetInv;
+        //   MultiSet5Slice(a[..], lo, target_i, right_i, hi);
+        // }
       }
+
+      // assert MultisetInv(a, cache, snap, lo, mid, hi, target_i, left_i, right_i) by {
+      assert multiset(a[..target_start]) + multiset(a[target_start..target_i]) + multiset(cache[left_i..left_bound]) + multiset(a[right_i..right_bound]) + multiset(a[target_bound..]) == multiset(snap) by {
+        ghost var snap_left_i := left_start;
+        ghost var snap_right_i := right_start;
+        ghost var snap_target_i := target_start;
+
+        ghost var snap_2 := snap;
+
+        assert multiset(snap_2[..target_start]) + multiset(snap_2[target_start..snap_target_i]) + multiset(snap_cache[snap_left_i..left_bound]) + multiset(snap_2[snap_right_i..right_bound]) + multiset(snap_2[target_bound..]) == multiset(snap) by {
+          assert snap[snap_target_i..snap_right_i] == snap_cache[snap_left_i..left_bound];
+          assert multiset(snap[snap_target_i..snap_right_i]) == multiset(snap_cache[snap_left_i..left_bound]);
+          MultiSet5Slice(snap_2, target_start, snap_target_i, snap_right_i, target_bound);
+        }
+
+        while snap_left_i < left_bound && snap_right_i < right_bound
+          // indices invariants
+          invariant left_start <= snap_left_i <= left_bound
+          invariant right_start <= snap_right_i <= right_bound
+          invariant (snap_left_i - left_start) + (snap_right_i - right_start) == (snap_target_i - target_start)
+          invariant target_start <= snap_target_i <= target_bound
+
+          invariant right_bound <= |snap_2|
+          invariant target_bound <= |snap_2|
+
+          // multiset invariant
+          invariant multiset(snap_2[..target_start]) + multiset(snap_2[target_start..snap_target_i]) + multiset(snap_cache[snap_left_i..left_bound]) + multiset(snap_2[snap_right_i..right_bound]) + multiset(snap_2[target_bound..]) == multiset(snap)
+        {
+          if leq(snap_cache[snap_left_i], snap[snap_right_i]) {
+            snap_2 := snap_2[snap_target_i := snap_cache[snap_left_i]];
+            snap_left_i := snap_left_i + 1;
+          } else {
+            snap_2 := snap_2[snap_target_i := snap_2[snap_right_i]];
+            snap_right_i := snap_right_i + 1;
+          }
+
+          snap_target_i := snap_target_i + 1;
+
+          assert multiset(snap_2[..target_start]) + multiset(snap_2[target_start..snap_target_i]) + multiset(snap_cache[snap_left_i..left_bound]) + multiset(snap_2[snap_right_i..right_bound]) + multiset(snap_2[target_bound..]) == multiset(snap) by {
+            assert snap[lo+snap_left_i..right_start] == snap_cache[snap_left_i..left_bound];
+            assert multiset(snap[lo+snap_left_i..right_start]) == multiset(snap_cache[snap_left_i..left_bound]);
+            MultiSet5Slice(snap_2, target_start, snap_target_i, snap_right_i, target_bound);
+          }
+        }
+      }
+
 
       // if right is exhausted copy left
       while left_i < left_bound
@@ -145,10 +236,17 @@ module BlockSortUnbound {
 
         //target
         invariant SortedBy(leq, a[target_start..target_i])
+
+        // invariant MultisetInv(a, cache, snap, lo, mid, hi, target_i, left_i, right_i)
       {
         a[target_i] := cache[left_i];
         left_i := left_i + 1;
         target_i := target_i + 1;
+
+        // assert MultisetInv(a, cache, snap, lo, mid, hi, target_i, left_i, right_i) by {
+        //   reveal MultisetInv;
+        //   MultiSet5Slice(a[..], lo, target_i, right_i, hi);
+        // }
       }
 
       // if left is exhausted assert goal by asserting right side is allready in place
@@ -182,6 +280,11 @@ module BlockSortUnbound {
           target_i := target_i + 1;
         }
       }
+
+      // assert multiset(a[..]) == multiset(snap) by {
+      //   reveal MultisetInv;
+      //   MultiSetTrippleSlice(a[..], lo, hi);
+      // }
     }
 
   }
@@ -189,5 +292,3 @@ module BlockSortUnbound {
 
 
 }
-
-
